POCs for net, java, python

TestModels/OrphanedShapes/runtimes/net/Extern/SimpleOrphanedShapesImpl_Compile.cs
@@ -1,0 +1,31 @@
+// Copyright Amazon.com Inc. or its affiliates. All Rights Reserved.
+// SPDX-License-Identifier: Apache-2.0
+using System;
+using Dafny;
+using simple.orphanedshapes.internaldafny.types;
+using Simple.OrphanedShapes;
+using Wrappers_Compile;
+
+namespace SimpleOrphanedShapesImpl_Compile
+{
+    public partial class __default
+    {
+        public static simple.orphanedshapes.internaldafny.types._IOrphanedStructure InitializeOrphanedStructure(simple.orphanedshapes.internaldafny.types._IOrphanedStructure input)
+        {
+            // .NET doesn't have this conversion
+            // Simple.OrphanedShapes.OrphanedStructure nativeStructure = TypeConversion.
+        }
+
+        public static simple.orphanedshapes.internaldafny.types._IOrphanedResource InitializeOrphanedStructure(simple.orphanedshapes.internaldafny.types._IOrphanedStructure input)
+        {
+            // .NET doesn't have this conversion
+            // Simple.OrphanedShapes.OrphanedStructure nativeStructure = TypeConversion.
+        }
+
+        public static simple.orphanedshapes.internaldafny.types._IOrphanedResource InitializeOrphanedStructure(simple.orphanedshapes.internaldafny.types._IOrphanedStructure input)
+        {
+            // .NET doesn't have this conversion
+            // Simple.OrphanedShapes.OrphanedStructure nativeStructure = TypeConversion.
+        }
+    }
+}
