TestModels/OrphanedShapes/runtimes/python/src/simple_orphaned_shapes/internaldafny/extern/SimpleOrphanedShapesImpl.py
@@ -1,0 +1,31 @@
+import simple_orphaned_shapes.internaldafny.generated.SimpleOrphanedShapesImpl
+from simple_orphaned_shapes.internaldafny.generated.SimpleOrphanedShapesImpl import *
+
+class default__(simple_orphaned_shapes.internaldafny.generated.SimpleOrphanedShapesImpl.default__):
+
+    @staticmethod
+    def InitializeOrphanedStructure(dafny_uninitialized_structure):
+        native_structure = simple_orphaned_shapes.smithygenerated.simple_orphanedshapes.dafny_to_smithy.simple_orphanedshapes_OrphanedStructure(dafny_uninitialized_structure)
+        native_structure.string_value = "the extern MUST use Smithy-generated conversions to set this value in the native structure"
+        dafny_initialized_structure = simple_orphaned_shapes.smithygenerated.simple_orphanedshapes.smithy_to_dafny.simple_orphanedshapes_OrphanedStructure(native_structure)
+        return dafny_initialized_structure
+
+    @staticmethod
+    def CallNativeOrphanedResource(dafny_resource):
+        native_resource = simple_orphaned_shapes.smithygenerated.simple_orphanedshapes.dafny_to_smithy.simple_orphanedshapes_OrphanedResourceReference(dafny_resource)
+        out = native_resource.orphaned_resource_operation(
+            simple_orphaned_shapes.smithygenerated.simple_orphanedshapes.models.OrphanedResourceOperationInput(
+                some_string = "the extern MUST provide this string to the native resource's operation"
+            )
+        )
+        dafny_resource_again = simple_orphaned_shapes.smithygenerated.simple_orphanedshapes.smithy_to_dafny.simple_orphanedshapes_OrphanedResourceReference(native_resource)
+        return dafny_resource_again
+
+    @staticmethod
+    def CallNativeOrphanedError(dafny_error):
+        native_error = simple_orphaned_shapes.smithygenerated.simple_orphanedshapes.deserialize._deserialize_error(dafny_error)
+        native_error.message = "the extern MUST use Smithy-generated conversions to set this value in the native error"
+        dafny_error_again = simple_orphaned_shapes.smithygenerated.simple_orphanedshapes.errors._smithy_error_to_dafny_error(native_error)
+        return dafny_error_again
+
+simple_orphaned_shapes.internaldafny.generated.SimpleOrphanedShapesImpl.default__ = default__
