TestModels/OrphanedShapes/runtimes/python/test/internaldafny/extern/wrapped_orphaned_resource.py
@@ -1,0 +1,7 @@
+from simple_orphaned_shapes.smithygenerated.simple_orphanedshapes.references import OrphanedResource
+
+class default__:
+    @staticmethod
+    def WrappedResource():
+        native_resource = OrphanedResource()
+        dafny_resource = simple_orphaned_shapes.smithygenerated.simple_orphanedshapes.smithy_to_dafny.
