TestModels/OrphanedShapes/runtimes/python/test/internaldafny/extern/wrapped_simple_orphaned_shapes.py
@@ -1,0 +1,22 @@
+# Copyright Amazon.com Inc. or its affiliates. All Rights Reserved.
+# SPDX-License-Identifier: Apache-2.0
+
+# src imports
+from simple_orphaned_shapes.smithygenerated.simple_orphanedshapes.client import SimpleOrphanedShapes
+from simple_orphaned_shapes.smithygenerated.simple_orphanedshapes.shim import SimpleOrphanedShapesShim
+from simple_orphaned_shapes.smithygenerated.simple_orphanedshapes.config import dafny_config_to_smithy_config
+import smithy_dafny_standard_library.internaldafny.generated.Wrappers as Wrappers
+
+# test imports, not qualified since this isn't in a package
+import WrappedSimpleOrphanedShapesService
+
+class default__(WrappedSimpleOrphanedShapesService.default__):
+
+    @staticmethod
+    def WrappedSimpleOrphanedShapes(config):
+        wrapped_config = dafny_config_to_smithy_config(config)
+        impl = SimpleOrphanedShapes(wrapped_config)
+        wrapped_client = SimpleOrphanedShapesShim(impl)
+        return Wrappers.Result_Success(wrapped_client)
+
+WrappedSimpleOrphanedShapesService.default__ = default__
