codegen/smithy-dafny-codegen/src/main/java/software/amazon/polymorph/smithypython/localservice/extensions/DirectedDafnyPythonLocalServiceCodegen.java
@@ -518,16 +518,16 @@ public class DirectedDafnyPythonLocalServiceCodegen
         // Neither classes nor converisons are generated for strings
       } else if (shapeToGenerate.isIntegerShape()) {
         // Neither classes nor converisons are generated for ints
-        continue;
       } else if (shapeToGenerate.isListShape()) {
         // Neither classes nor converisons are generated for lists
-        continue;
       } else if (shapeToGenerate.isMapShape()) {
         // Neither classes nor converisons are generated for maps
-        continue;
       } else if (shapeToGenerate.isLongShape()) {
         // Neither classes nor converisons are generated for longs
-        continue;
+      } else if (shapeToGenerate.isBlobShape()) {
+        // Neither classes nor converisons are generated for blobs
+      } else if (shapeToGenerate.isBooleanShape()) {
+        // Neither classes nor converisons are generated for blobs
       } else {
         // Add more as needed...
         throw new ClassCastException(
