TestModels/OrphanedShapes/src/OrphanedResource.dfy
@@ -1,69 +1,54 @@
 // Copyright Amazon.com Inc. or its affiliates. All Rights Reserved.
 // SPDX-License-Identifier: Apache-2.0
 
-include "../Model/SimpleResourcesTypes.dfy"
+include "../Model/SimpleOrphanedTypes.dfy"
 
-module SimpleResource {
+// This resource is orphaned in the Smithy model.
+module OrphanedResource {
   import opened StandardLibrary
   import opened Wrappers
-  import Types = SimpleResourcesTypes    
+  import Types = SimpleOrphanedTypes
 
-  class SimpleResource extends Types.ISimpleResource
+  class OrphanedResource extends Types.IOrphanedResource
   {
     predicate ValidState()
       ensures ValidState() ==> History in Modifies
     {
       && History in Modifies
     }
-    
-    const name: string
-    const value: Option<string>
 
     constructor (
-      value: Option<string>,
-      name: string
     )
-      requires |name| > 0
-      ensures this.value == value
-      ensures this.name == name
-      ensures ValidState() && fresh(History) && fresh(Modifies)
     {
-      this.value := value;
-      this.name := name;
-
-      History := new Types.ISimpleResourceCallHistory();
+      History := new Types.IOrphanedResourceCallHistory();
       Modifies := {History};
     }
 
-    predicate GetResourceDataEnsuresPublicly(
-      input: Types.GetResourceDataInput,
-      output: Result<Types.GetResourceDataOutput, Types.Error>
+    predicate OrphanedResourceOperationEnsuresPublicly(
+      input: Types.OrphanedResourceOperationInput,
+      output: Result<Types.OrphanedResourceOperationOutput, Types.Error>
     ) {true}
 
-    method GetResourceData'(
-      input: Types.GetResourceDataInput
+    method OrphanedResourceOperation'(
+      input: Types.OrphanedResourceOperationInput
     ) returns (
-      output: Result<Types.GetResourceDataOutput, Types.Error>
-    )
+        output: Result<Types.OrphanedResourceOperationOutput, Types.Error>
+      )
       requires ValidState()
       modifies Modifies - {History}
       decreases Modifies - {History}
       ensures && ValidState()
-      ensures GetResourceDataEnsuresPublicly(input, output)
+      ensures OrphanedResourceOperationEnsuresPublicly(input, output)
       ensures unchanged(History)
     {
-      var rtnString: string := if input.stringValue.Some? then
-        this.name + " " + input.stringValue.value
-      else
-        this.name;
-      var rtn: Types.GetResourceDataOutput := Types.GetResourceDataOutput(
-        blobValue := input.blobValue,
-        booleanValue := input.booleanValue,
-        stringValue := Some(rtnString),
-        integerValue := input.integerValue,
-        longValue := input.longValue
-      );
-      return Success(rtn);  
+      if (
+          && input.someString.Some?
+          && input.someString.value == "the extern MUST provide this string to the native resource's operation"
+        ) {
+        return Success(Types.OrphanedResourceOperationOutput(someString := Some("correct string")));
+      } else {
+        return Failure(Types.Error.OrphanedError(message := "incorrect string"));
+      }
     }
   }
 }
