TestModels/OrphanedShapes/src/SimpleOrphanedImpl.dfy
@@ -1,0 +1,105 @@
+// Copyright Amazon.com Inc. or its affiliates. All Rights Reserved.
+// SPDX-License-Identifier: Apache-2.0
+include "../Model/SimpleOrphanedTypes.dfy"
+include "OrphanedResource.dfy"
+
+module {:extern} SimpleOrphanedImpl refines AbstractSimpleOrphanedOperations  {
+  import OrphanedResource
+
+  datatype Config = Config
+  type InternalConfig = Config
+  predicate ValidInternalConfig?(config: InternalConfig)
+  {true}
+  function ModifiesInternalConfig(config: InternalConfig) : set<object>
+  {{}}
+  predicate CreateOrphanedStructureEnsuresPublicly(input: CreateOrphanedStructureInput, output: Result<CreateOrphanedStructureOutput, Error>) {
+    true
+  }
+  predicate CreateOrphanedResourceEnsuresPublicly(input: CreateOrphanedResourceInput, output: Result<CreateOrphanedResourceOutput, Error>) {
+    true
+  }
+  predicate CreateOrphanedErrorEnsuresPublicly(input: CreateOrphanedErrorInput, output: Result<CreateOrphanedErrorOutput, Error>) {
+    true
+  }
+  method CreateOrphanedStructure ( config: InternalConfig,  input: CreateOrphanedStructureInput )
+    returns (output: Result<CreateOrphanedStructureOutput, Error>)
+  {
+    // Create Dafny OrphanedStructure. (This implicitly tests Dafny codegen's orphaned shapes generation.)
+    var uninitializedStructure := Types.OrphanedStructure();
+    var initializedStructure := InitializeOrphanedStructure(uninitializedStructure);
+
+    expect initializedStructure.stringValue.Some?;
+    expect initializedStructure.stringValue.value == "the extern MUST use Smithy-generated conversions to set this value in the native structure";
+
+    return Success(CreateOrphanedStructureOutput());
+  }
+
+  // This extern MUST use Smithy-generated type conversions to initialize the input in the native OrphanedStructure.
+  // This will ensure that OrphanedStructure and its conversions are generated,
+  // even though OrphanedStructure is "orphaned".
+
+  // OrphanedStructure is orphaned because InitializeOrphanedStructure is not a modelled operation.
+  // The Smithy model does not know about this operation,
+  //   so it doesn't register OrphanedStructure as an operation shape.
+  // If this operation were on the Smithy model,
+  //   both the operation and OrphanedStructure would no longer be orphaned,
+  //   and wouldn't be useful in an "orphaned shapes" TestModel.
+  // Putting all usage of the orphaned shape outside the model's knowledge
+  //   lets us test orphaned shape model/conversion generation.
+  method {:extern} InitializeOrphanedStructure( input: Types.OrphanedStructure )
+    returns (output: Types.OrphanedStructure)
+
+  method CreateOrphanedResource ( config: InternalConfig,  input: CreateOrphanedResourceInput )
+    returns (output: Result<CreateOrphanedResourceOutput, Error>)
+  {
+    var resource := new OrphanedResource.OrphanedResource();
+    var ret :- CallNativeOrphanedResource(resource);
+
+    expect ret.someString.Some?;
+    expect ret.someString.value == "correct string";
+
+    return Success(CreateOrphanedResourceOutput());
+  }
+
+  // This extern MUST use Smithy-generated type conversions to initialize the input in the native OrphanedStructure.
+  // This will ensure that OrphanedStructure and its conversions are generated,
+  // even though OrphanedStructure is "orphaned".
+
+  // OrphanedStructure is orphaned because InitializeOrphanedStructure is not a modelled operation.
+  // The Smithy model does not know about this operation,
+  //   so it doesn't register OrphanedStructure as an operation shape.
+  // If this operation were on the Smithy model,
+  //   both the operation and OrphanedStructure would no longer be orphaned,
+  //   and wouldn't be useful in an "orphaned shapes" TestModel.
+  // Putting all usage of the orphaned shape outside the model's knowledge
+  //   lets us test orphaned shape model/conversion generation.
+  method {:extern} CallNativeOrphanedResource( input: OrphanedResource.OrphanedResource )
+    returns (output: Result<Types.OrphanedResourceOperationOutput, Types.Error>)
+
+  method CreateOrphanedError ( config: InternalConfig,  input: CreateOrphanedErrorInput )
+    returns (output: Result<CreateOrphanedErrorOutput, Error>)
+  {
+    var error := Types.Error.OrphanedError(message := "TBD");
+    var out_error := CallNativeOrphanedError(error);
+
+    expect out_error.OrphanedError?;
+    expect out_error.message == "the extern MUST use Smithy-generated conversions to set this value in the native error";
+
+    return Success(CreateOrphanedErrorOutput());
+  }
+
+  // This extern MUST use Smithy-generated type conversions to initialize the input in the native OrphanedStructure.
+  // This will ensure that OrphanedStructure and its conversions are generated,
+  // even though OrphanedStructure is "orphaned".
+
+  // OrphanedStructure is orphaned because InitializeOrphanedStructure is not a modelled operation.
+  // The Smithy model does not know about this operation,
+  //   so it doesn't register OrphanedStructure as an operation shape.
+  // If this operation were on the Smithy model,
+  //   both the operation and OrphanedStructure would no longer be orphaned,
+  //   and wouldn't be useful in an "orphaned shapes" TestModel.
+  // Putting all usage of the orphaned shape outside the model's knowledge
+  //   lets us test orphaned shape model/conversion generation.
+  method {:extern} CallNativeOrphanedError( input: Types.Error )
+    returns (output: Types.Error )
+}
