TestModels/OrphanedShapes/test/WrappedTest.dfy
@@ -1,28 +1,48 @@
 // Copyright Amazon.com Inc. or its affiliates. All Rights Reserved.
 // SPDX-License-Identifier: Apache-2.0
 
-include "../src/WrappedIndex.dfy"
-include "./SimpleResourcesTest.dfy"
+include "../src/WrappedSimpleOrphanedImpl.dfy"
+
+// There are no non-wrapped tests for this TestModel.
+// This TestModel requires implementing externs that call Polymorph-generated code.
+// Polymorph must be in the mix, even for the non-wrapped client, so it is reasonable to only have wrapped tests.
 
 module WrappedTest {
-  import opened SimpleResourcesTest
-  import WrappedSimpleResources
-  import opened Types = SimpleResourcesTypes
-  import opened Wrappers
+  import WrappedSimpleOrphanedService
+  import opened Types = SimpleOrphanedTypes
 
-  method TestWrappedClient(config: Types.SimpleResourcesConfig)
+  method {:test} TestWrappedClient()
   {
-    var client :- expect WrappedSimpleResources.WrappedSimpleResources(config);
-    var resource := TestGetResources(config, client);
-    TestNoneGetData(config, resource);
-    TestSomeGetData(config, resource);
-  }
-  
-  method {:test} WrappedTestDefaultConfig() {
-    TestWrappedClient(WrappedSimpleResources.WrappedDefaultSimpleResourcesConfig());
+    var client :- expect WrappedSimpleOrphanedService.WrappedSimpleOrphaned();
+    TestCreateOrphanedStructure(client);
+    TestCreateOrphanedResource(client);
+    TestCreateOrphanedError(client);
   }
 
-  method {:test} WrappedTestCustomConfig() {
-    TestWrappedClient(Types.SimpleResourcesConfig(name := "Dafny"));
+  method TestCreateOrphanedStructure(client: Types.ISimpleOrphanedClient)
+      requires client.ValidState()
+      modifies client.Modifies
+      ensures client.ValidState()
+  {
+    var ret := client.CreateOrphanedStructure(Types.CreateOrphanedStructureInput);
+    expect ret.Success?;
+  }
+
+    method TestCreateOrphanedResource(client: Types.ISimpleOrphanedClient)
+      requires client.ValidState()
+      modifies client.Modifies
+      ensures client.ValidState()
+  {
+    var ret := client.CreateOrphanedResource(Types.CreateOrphanedResourceInput);
+    expect ret.Success?;
+  }
+
+  method TestCreateOrphanedError(client: Types.ISimpleOrphanedClient)
+      requires client.ValidState()
+      modifies client.Modifies
+      ensures client.ValidState()
+  {
+    var ret := client.CreateOrphanedError(Types.CreateOrphanedErrorInput);
+    expect ret.Success?;
   }
 }
