TestModels/OrphanedShapes/README.md
@@ -1,0 +1,54 @@
+# OrphanedShapes
+
+## Background
+
+This project tests for support of "orphaned" shapes.
+
+An "orphaned" is a shape that exists in a Smithy model, but is not discovered by Smithy-Core's shape discovery logic.
+
+Smithy-Core will only discover and generate code for shapes that are attached to a service via the service's
+1. Operations
+2. Mixins
+3. Errors
+
+and recursive traversals of the connected shapes.
+
+If a shape is defined in a Smithy model,
+but not declared in a LocalService's operations or errors
+(or recursive traversals of these),
+codegens that use Smithy-Core's shape discovery will not generate code for the shape.
+(Similar for mixins, but Polymorph doesn't have any usage of these at the moment.)
+
+Smithy-Dafny .NET and Java generate code for orphaned shapes because these codegens don't use Smithy-Core's shape discovery logic.
+
+By default, any language extending a "real" Smithy code generator use Smithy-Core's shape discovery logic, and do not support orphaned shapes.
+
+The expectation is that code is generated for orphaned shapes.
+The generated code must include any class definitions and Dafny/native conversions.
+
+## Prerequisites
+
+This TestModel assumes these other TestModels are passing:
+
+- Extern
+- Extendable
+- LocalService
+- Union
+- Aggregate
+- Enum
+
+and these TestModels' prerequisite TestModels.
+
+## Coverage
+
+This TestModel tests some instances of orphaned shapes
+- LocalService Config shapes. These are "orphaned", but are likely already handled as one-offs by any codegen that's this TestModels' prerequisites.
+- Errors
+- Resources (with @aws.polymorph#reference trait) and their operations
+- Structures (and structures' members)
+
+The "key" to this TestModel is in the extern implementations.
+The externs require passing some orphaned shapes across the Dafny layer.
+The extern implementations MUST call Polymorph-generated native shapes and Dafny/native conversions for these orphaned shapes.
+However, Polymorph will only generate these shapes and conversions if the language's codegen supports orphaned shapes.
+So if this language generates these conversions, then it supports orphaned shapes.
